Upd: fix typeclass set and improve structure throughout project

theories/ATPCompat.v
@@ -2,10 +2,16 @@
 
 From Corelib Require Import Classes.RelationClasses.
 
+From Stdlib Require Import Classical.
+From Stdlib Require Import Lia.
+
 From Tableaux Require Import Syntax.
 From Tableaux Require Import Semantics.
 From Tableaux Require Import Proofs.
 From Tableaux Require Import Skolemization.
+
+Export ConcreteSyntaxInstances.
+Export ConcreteSkolemizationInstances.
 
 (** In this file, we define:
       1. a syntax using [string]s for bound variable, in order to make it easy to
@@ -90,8 +96,8 @@ Section ESemantics.
       | EPred p l => interp_pred p (map (interpret_eterm rho) l)
       | ENeg F    => ~ (rec rho F)
       | EOr F G   => rec rho F \/ rec rho G
-      | EAnd F G  => rec rho F \/ rec rho G
-      | EImp F G  => ~(rec rho F) \/ rec rho G
+      | EAnd F G  => rec rho F /\ rec rho G
+      | EImp F G  => rec rho F -> rec rho G
       | EEqu F G  => rec rho F <-> rec rho G
       | EEx x F   => exists (v : M), rec (fun y => match eqDec x y with
                                           | left _ => Some v
@@ -112,21 +118,44 @@ Section ESyntaxTranslation.
   Fixpoint fv_eterm (t : ETerm) : SetOfString :=
     match t with
     | EVar x   => singleton x
-    | EFun f l => fold_left (fun s t => s \union (fv_eterm t)) l (empty_set string)
+    | EFun f l => fold_left (fun s t => s \union (fv_eterm t)) l empty_set
     end.
 
-  Fixpoint fv_eform (F : EForm) : SetOfString :=
+  Lemma fv_efun :
+    forall (f : string) (l : list ETerm) (t : ETerm) (x : string),
+      In t l -> mem x (fv_eterm t) -> mem x (fv_eterm (EFun f l)).
+  Proof.
+    intros ???? hin hmem. cbn[fv_eterm] in hmem |- *.
+    induction l as [|y ys IHys].
+    - inversion hin.
+    - rewrite mem_fold_left_cons_unionl. apply union_spec. destruct hin as [hin | e].
+      + left. now apply IHys.
+      + right. rewrite -e //.
+  Qed.
+
+  (* Fixpoint fv_eform (F : EForm) : SetOfString := *)
+  (*   match F with *)
+  (*   | EBot | ETop => empty_set string *)
+  (*   | EPred p l => fold_left (fun s t => s \union (fv_eterm t)) l (empty_set string) *)
+  (*   | ENeg F => fv_eform F *)
+  (*   | EOr F G | EAnd F G | EImp F G | EEqu F G => (fv_eform F) \union (fv_eform G) *)
+  (*   | EEx x F | EAll x F => remove x (fv_eform F) *)
+  (*   end. *)
+
+  Fixpoint bv_eform (F : EForm) : SetOfString :=
     match F with
-    | EBot | ETop => empty_set string
-    | EPred p l => fold_left (fun s t => s \union (fv_eterm t)) l (empty_set string)
-    | ENeg F => fv_eform F
-    | EOr F G | EAnd F G | EImp F G | EEqu F G => (fv_eform F) \union (fv_eform G)
-    | EEx x F | EAll x F => remove x (fv_eform F)
+    | EBot | ETop | EPred _ _ => empty_set
+    | ENeg F => bv_eform F
+    | EOr F G | EAnd F G | EImp F G | EEqu F G => (bv_eform F) \union (bv_eform G)
+    | EEx x F | EAll x F => add x (bv_eform F)
     end.
 
-  Definition WellScoped (F : EForm) := is_empty (fv_eform F).
+  (* Definition WellScoped (F : EForm) := is_empty (fv_eform F). *)
 
-  Fixpoint index_of {A : Type} `{EqDec A} (x : A) (l : list A) : option nat :=
+  Section IndexOf.
+    Context {A : Type} `{EqDec A}.
+
+    Fixpoint index_of (x : A) (l : list A) : option nat :=
     match l with
     | [] => None
     | y :: ys => match eqDec x y with
@@ -134,6 +163,124 @@ Section ESyntaxTranslation.
                | right _ => bind (index_of x ys) (fun n => Some (S n))
                end
     end.
+
+    Lemma index_of_spec :
+      forall (x : A) (n : nat) (l : list A),
+        index_of x l = Some n -> nth_error l n = Some x.
+    Proof using Type.
+      intros ??? e. generalize dependent n. induction l as [|y ys IHys].
+      - intros ? e. inversion e.
+      - intros ? e; cbn in *. destruct eqDec; cbn.
+        + injection e => <-. cbn. rewrite e0 //.
+        + destruct (index_of x ys) eqn:eid; cbn in *.
+          * injection e => en. rewrite -en; cbn.
+            now apply IHys.
+          * inversion e.
+    Qed.
+
+    Lemma index_of_inj :
+      forall (x y : A) (n : nat) (l : list A),
+        index_of x l = Some n -> index_of y l = Some n -> x = y.
+    Proof using Type.
+      intros ???? ex ey. generalize dependent n; induction l as [|z zs IHzs]; intros n ex ey.
+      - inversion ex.
+      - cbn in *. repeat (destruct eqDec; cbn in * ).
+        + now rewrite e0.
+        + rewrite -ex in ey. destruct (index_of y zs); cbn in *.
+          * injection ey => contra; inversion contra.
+          * inversion ey.
+        + rewrite -ey in ex. destruct (index_of x zs); cbn in *.
+          * injection ex => contra; inversion contra.
+          * inversion ex.
+        + destruct n.
+          * destruct (index_of x zs), (index_of y zs); cbn in *.
+            -- injection ex => contra; inversion contra.
+            -- inversion ey.
+            -- inversion ex.
+            -- inversion ex.
+          * destruct (index_of x zs), (index_of y zs); cbn in *.
+            -- apply (IHzs n); f_equal.
+               ++ apply eq_add_S. now injection ex => ->.
+               ++ apply eq_add_S. now injection ey => ->.
+            -- inversion ey.
+            -- inversion ex.
+            -- inversion ex.
+    Qed.
+
+    Lemma In_index_of :
+      forall (x : A) (l : list A), In x l -> exists (n : nat), index_of x l = Some n.
+    Proof using Type.
+      intros x l hin. induction l as [|y ys IHys].
+      - inversion hin.
+      - cbn. destruct (x == y).
+        + now exists 0.
+        + destruct hin as [hin | e].
+          * apply IHys in hin. destruct hin as [m e].
+            exists (S m). destruct (index_of x ys).
+            -- cbn. injection e => -> //.
+            -- inversion e.
+          * exfalso. now apply n.
+    Qed.
+
+    Lemma index_of_In :
+      forall (x : A) (l : list A) (n : nat), index_of x l = Some n -> In x l.
+    Proof using Type.
+      intros ??. induction l as [|y ys IHys].
+      - intros ? contra; inversion contra.
+      - intros ? e; cbn in *. destruct (x == y).
+        + now right.
+        + left. destruct (index_of x ys); cbn in *.
+          * injection e => e'. destruct n.
+            -- inversion e'.
+            -- apply (IHys n). f_equal. now apply eq_add_S.
+          * inversion e.
+    Qed.
+
+    Lemma index_of_cons :
+      forall (x y : A) (l : list A) (n : nat),
+        index_of x (y :: l) = Some (S n) -> index_of x l = Some n.
+    Proof using Type.
+      intros ???? e; cbn in *.
+      destruct (x == y); cbn.
+      - injection e => contra. inversion contra.
+      - destruct (index_of x l); cbn in *.
+        + f_equal. apply eq_add_S. now injection e => ->.
+        + inversion e.
+    Qed.
+
+    Lemma index_of_cons' :
+      forall (x y : A) (l : list A) (n : nat),
+        x <> y -> index_of x l = Some n -> index_of x (y :: l) = Some (S n).
+    Proof using Type.
+      intros ???? e0 e; cbn in *.
+      destruct (x == y); cbn.
+      - congruence.
+      - destruct (index_of x l); cbn in *.
+        + f_equal. apply eq_S. injection e => -> //.
+        + inversion e.
+    Qed.
+
+    Lemma index_of_nth :
+      forall (x : A) (l1 l2 : list A),
+        (forall (n : nat), n < min #|l1| #|l2| -> nth_error l1 n = nth_error l2 n) ->
+        In x l1 -> In x l2 ->
+        index_of x l1 = index_of x l2.
+    Proof using Type.
+      intros ??. induction l1 as [|y ys IHys].
+      - intros []; auto. intros _ contra; inversion contra.
+      - intros [].
+        + intros _ _ contra; inversion contra.
+        + intros h hin hin'. cbn. destruct (x == y), (x == a); auto.
+          * specialize (h 0). cbn in h. specialize (h ltac:(lia)).
+            injection h => contra; congruence.
+          * specialize (h 0). cbn in h. specialize (h ltac:(lia)).
+            injection h => contra; congruence.
+          * rewrite (IHys l); auto.
+            -- intros. specialize (h (S n1)). cbn in h. now specialize (h ltac:(lia)).
+            -- destruct hin; congruence.
+            -- destruct hin'; congruence.
+    Qed.
+  End IndexOf.
 
   Fixpoint translate_ETerm (m : list string) (t : ETerm) : Term :=
     match t with
@@ -195,29 +342,252 @@ Section ESyntaxTranslation.
                    end)
     end.
 
-  Lemma WellScoped_no_fv_eterm :
-    forall (t : ETerm), is_empty (fv_eterm t) -> is_empty (@fv string _ _ (translate_ETerm [] t)).
-  Proof.
-    intros t hscope; induction t using eterm_rect'; cbn in *.
-    - assumption.
-    - induction l.
-      + now cbn in *.
-      + cbn in *. Admitted.
+  (* Lemma WellScoped_no_fv_eterm : *)
+  (*   forall (t : ETerm), is_empty (fv_eterm t) -> is_empty (@fv string _ _ (translate_ETerm [] t)). *)
+  (* Proof. *)
+  (*   intros t hscope; induction t using eterm_rect'; cbn in *. *)
+  (*   - assumption. *)
+  (*   - induction l. *)
+  (*     + now cbn in *. *)
+  (*     + cbn in *. Admitted. *)
 
-  Lemma WellScoped_no_fv :
-    forall (F : EForm), WellScoped F -> is_empty (@fv string _ _ (translate_EForm F)).
+  (* Lemma WellScoped_no_fv : *)
+  (*   forall (F : EForm), WellScoped F -> is_empty (@fv string _ _ (translate_EForm F)). *)
+  (* Proof. *)
+  (*   intros F hscope; induction F. *)
+  (*   - cbn. rewrite is_empty_spec //. *)
+  (*   - cbn; rewrite is_empty_spec //. *)
+  (*   - cbn in *. admit. *)
+  (*   - cbn in *. now apply IHF. *)
+  (*   - admit. *)
+  (*   - admit. *)
+  (*   - admit. *)
+  (*   - admit. *)
+  (*   - admit. *)
+  (*   - admit. *)
+  (* Admitted. *)
+
+  (* Definition LocallyClosedETerm (t : ETerm) (rho : list string) := *)
+  (*   forall (x : string), mem x (fv_eterm t) -> (In x rho -> False). *)
+
+  (* Lemma LocallyClosed_tail : *)
+  (*   forall (t : ETerm) (x : string) (rho : list string), *)
+  (*     LocallyClosedETerm t (x :: rho) -> LocallyClosedETerm t rho. *)
+  (* Proof. intros ??? hclosed y hmem hin. eapply hclosed; eauto. now left. Qed. *)
+
+  (* Lemma LocallyClosedETerm_translate_all : *)
+  (*   forall (t : ETerm) (rho sigma : list string), *)
+  (*     LocallyClosedETerm t rho -> LocallyClosedETerm t sigma -> *)
+  (*     translate_ETerm rho t = translate_ETerm sigma t. *)
+  (* Proof. *)
+  (*   intros ??? closedr closeds. induction t using eterm_ind. *)
+  (*   - red in closedr, closeds. cbn[fv_eterm] in closedr, closeds. *)
+  (*     specialize (closedr x (singleton_spec x)). *)
+  (*     specialize (closeds x (singleton_spec x)). *)
+  (*     cbn. destruct (index_of x rho) eqn:xrho, (index_of x sigma) eqn:xsig. *)
+  (*     + now apply index_of_In, closedr in xrho. *)
+  (*     + now apply index_of_In, closedr in xrho. *)
+  (*     + now apply index_of_In, closeds in xsig. *)
+  (*     + reflexivity. *)
+  (*   - cbn. f_equal. *)
+  (*     have hr : forall (t : ETerm), In t l -> LocallyClosedETerm t rho. { *)
+  (*       clear H closeds. intros t hin x hmem hin'. *)
+  (*       specialize (closedr x). cbn[fv_eterm] in closedr. *)
+  (*       apply fv_efun with (f := f) (l := l) in hmem; auto. *)
+  (*     } *)
+  (*     have hs : forall (t : ETerm), In t l -> LocallyClosedETerm t sigma. { *)
+  (*       clear H closedr. intros t hin x hmem hin'. *)
+  (*       specialize (closeds x). cbn[fv_eterm] in closeds. *)
+  (*       apply fv_efun with (f := f) (l := l) in hmem; auto. *)
+  (*     } *)
+  (*     have H' : forall (t : ETerm), In t l -> translate_ETerm rho t = translate_ETerm sigma t. { *)
+  (*       intros. apply Forall_In with (x := t) in H; auto. *)
+  (*     } *)
+  (*     clear closedr closeds H. *)
+  (*     induction l as [|x xs IHxs]; auto. *)
+  (*     cbn. rewrite H'. *)
+  (*     + now right. *)
+  (*     + rewrite IHxs; auto. *)
+  (*       * intros; apply hr. now left. *)
+  (*       * intros; apply hs. now left. *)
+  (*       * intros; apply H'. now left. *)
+  (* Qed. *)
+
+  (* Lemma instantiate_commutes_term : *)
+  (*   forall (t : ETerm) (x : string) (u : ETerm) (rho sigma : list string) (n : nat), *)
+  (*     (LocallyClosedETerm u rho /\ LocallyClosedETerm u sigma) -> *)
+  (*     index_of x rho = Some n  -> *)
+  (*     translate_ETerm rho (instantiate_eterm x u t) = *)
+  (*       (translate_ETerm rho t){n \to translate_ETerm sigma u}. *)
+  (* Proof. *)
+  (*   intros t; induction t using eterm_ind. *)
+  (*   - intros y ???? [closedr closeds] e; cbn. destruct eqDec; cbn. *)
+  (*     + destruct (index_of x rho) eqn:index; cbn. *)
+  (*       * destruct (eq_dec_nat n n0) eqn:enat; auto. *)
+  (*         subst. rewrite e in index. *)
+  (*         2: congruence. *)
+  (*         apply LocallyClosedETerm_translate_all; auto. *)
+  (*       * subst. rewrite e in index. inversion index. *)
+  (*     + destruct (index_of x rho) eqn:index; cbn; auto. *)
+  (*       destruct (eq_dec_nat n n1) eqn:enat; auto. *)
+  (*       rewrite -e0 in index. *)
+  (*       have ex : x = y. { eapply index_of_inj; eauto. } *)
+  (*       congruence. *)
+  (*   - intros; cbn. rewrite !map_map. *)
+  (*     have hmap : map (fun t => translate_ETerm rho (instantiate_eterm x u t)) l = *)
+  (*                   map (fun t => (translate_ETerm rho t){n \to translate_ETerm sigma u}) l. *)
+  (*     { induction l as [|y ys IHys]; auto. *)
+  (*       cbn. rewrite IHys. *)
+  (*       - now apply Forall_tail in H. *)
+  (*       - apply Forall_In with (x := y) in H. *)
+  (*         + erewrite H. *)
+  (*           2,3: eassumption. *)
+  (*           reflexivity. *)
+  (*         + now right. } *)
+  (*     rewrite hmap //. *)
+  (* Qed. *)
+
+  (* Lemma WellScoped_instantiate_commutes : *)
+  (*   forall (F : EForm) (x : string) (rho : list string) (sigma : list string) (t : ETerm) (n : nat), *)
+  (*     (forall (y : string), mem y (fv_eterm t) -> ~(mem y (bv_eform F))) -> *)
+  (*     LocallyClosedETerm t (x :: rho) -> LocallyClosedETerm t sigma -> index_of x rho = Some n -> *)
+  (*     translate_EForm_ rho (instantiate_eform x t F) = *)
+  (*       (translate_EForm_ rho F){n \to translate_ETerm sigma t}. *)
+  (* Proof. *)
+  (*   intros F x rho sigma t. revert rho sigma. induction F; auto; intros rho sigma n hclosedF hclosedr hcloseds e; *)
+  (*     cbn. *)
+  (*   - rewrite !map_map. *)
+  (*     have hmap : map (fun u => translate_ETerm rho (instantiate_eterm x t u)) l = *)
+  (*                   map (fun u => (translate_ETerm rho u){n \to translate_ETerm sigma t}) l. *)
+  (*     { induction l as [|y ys IHys]; auto. *)
+  (*       cbn. erewrite instantiate_commutes_term. *)
+  (*       3: eassumption. *)
+  (*       2: { apply LocallyClosed_tail in hclosedr; split; eauto. } *)
+  (*       rewrite IHys //. } *)
+  (*     rewrite hmap //. *)
+  (*   - erewrite IHF; eauto. *)
+  (*   - erewrite IHF1, IHF2; eauto. *)
+  (*     + intros y hmem hmem'.  apply (hclosedF y); auto. *)
+  (*       rewrite mem_union; now right. *)
+  (*     + intros y hmem hmem'.  apply (hclosedF y); auto. *)
+  (*       rewrite mem_union; now left. *)
+  (*   - erewrite IHF1, IHF2; eauto. *)
+  (*     + intros y hmem hmem'.  apply (hclosedF y); auto. *)
+  (*       rewrite mem_union; now right. *)
+  (*     + intros y hmem hmem'.  apply (hclosedF y); auto. *)
+  (*       rewrite mem_union; now left. *)
+  (*   - erewrite IHF1, IHF2; eauto. *)
+  (*     + intros y hmem hmem'.  apply (hclosedF y); auto. *)
+  (*       rewrite mem_union; now right. *)
+  (*     + intros y hmem hmem'.  apply (hclosedF y); auto. *)
+  (*       rewrite mem_union; now left. *)
+  (*   - erewrite IHF1, IHF2; eauto. *)
+  (*     + intros y hmem hmem'.  apply (hclosedF y); auto. *)
+  (*       rewrite mem_union; now right. *)
+  (*     + intros y hmem hmem'.  apply (hclosedF y); auto. *)
+  (*       rewrite mem_union; now left. *)
+  (*   - destruct (x == s); cbn. *)
+  (*     + rewrite e0. *)
+  (*       have en : n = 0. { admit. } (* todo: easy *) *)
+  (*       rewrite !en in e |- *. admit. (* yes: overshadowed *) *)
+  (*     + rewrite -(IHF (s :: rho) sigma (n + 1)); auto. *)
+  (*       * intros y hmem hmem'. apply (hclosedF y); auto. *)
+  (*         (* todo: mem_add *) admit. *)
+  (*       * intros y hmem hin. repeat destruct hin as [hin | e0]. *)
+  (*         -- apply (hclosedr y); auto. now left. *)
+  (*         -- apply (hclosedF y); auto. *)
+  (*            (* todo: mem_add *) admit. *)
+  (*         -- apply (hclosedr y); auto. now right. *)
+  (*       * rewrite PeanoNat.Nat.add_1_r; apply index_of_cons'; auto. *)
+  (*   - destruct (x == s); cbn. *)
+  (*     + rewrite e0. *)
+  (*       have en : n = 0. { admit. } (* todo: easy *) *)
+  (*       rewrite !en in e |- *. admit. (* yes: overshadowed *) *)
+  (*     + rewrite -(IHF (s :: rho) sigma (n + 1)); auto. *)
+  (*       * intros y hmem hmem'. apply (hclosedF y); auto. *)
+  (*         (* todo: mem_add *) admit. *)
+  (*       * intros y hmem hin. repeat destruct hin as [hin | e0]. *)
+  (*         -- apply (hclosedr y); auto. now left. *)
+  (*         -- apply (hclosedF y); auto. *)
+  (*            (* todo: mem_add *) admit. *)
+  (*         -- apply (hclosedr y); auto. now right. *)
+  (*       * rewrite PeanoNat.Nat.add_1_r; apply index_of_cons'; auto. *)
+  (*   Admitted. *)
+
+(* Pred s *)
+(*     (map (fun t : Term_ string string => t {#| rho | - 1 \to Free x}) (map (translate_ETerm rho) l)) = *)
+  (*   Pred s (map (translate_ETerm sigma) l) *)
+  Lemma instantiate_var_as_free_in_term :
+    forall (t : ETerm) (rho sigma : list string) (s : string) (n : nat),
+      index_of s rho = Some n ->
+      (forall m, m < n -> nth_error rho m = nth_error sigma m) ->
+      nth_error sigma n = None ->
+      (translate_ETerm rho t) {n \to Free s} = translate_ETerm sigma t.
   Proof.
-    intros F hscope; induction F.
-    - cbn. rewrite is_empty_spec //.
-    - cbn; rewrite is_empty_spec //.
-    - cbn in *. admit.
-    - cbn in *. now apply IHF.
-    - admit.
-    - admit.
-    - admit.
-    - admit.
-    - admit.
-    - admit.
+    intros t; induction t using eterm_ind'; intros rho sigma s n es erho hnone.
+    - cbn; destruct (index_of x rho) eqn:ex.
+      + destruct (index_of x sigma) eqn:ex'.
+        * cbn. destruct (n == n0).
+          -- subst. apply index_of_inj with (x := x) in es; auto.
+             subst. have h : index_of s rho = index_of s sigma.
+             { apply index_of_nth.
+               - intros. apply erho.
+                 have hlt : #|sigma| <= n0 by now rewrite nth_error_None in hnone.
+                 lia.
+               - now apply index_of_In in ex.
+               - now apply index_of_In in ex'. }
+             have e : n0 = n1 by congruence.
+             rewrite e in hnone. apply index_of_spec in ex'. congruence.
+          -- have h : index_of x rho = index_of x sigma.
+             { apply index_of_nth.
+               - intros. apply erho.
+                 have hlt : #|sigma| <= n by now rewrite nth_error_None in hnone. lia.
+               - now apply index_of_In in ex.
+               - now apply index_of_In in ex'. }
+             congruence.
+        * cbn. Admitted.
+
+  Lemma instantiate_var_as_free_in_form :
+    forall (F : EForm) (rho sigma : list string) (s : string) (n : nat),
+      index_of s rho = Some n ->
+      (forall m, m < n -> nth_error rho m = nth_error sigma m) ->
+      nth_error sigma n = None ->
+      (translate_EForm_ rho F) {n \to Free s} = translate_EForm_ sigma F.
+  Proof.
+    intros F; induction F; intros rho sigma x n ex erho hnone; cbn; auto.
+    - rewrite map_map. f_equal. induction l as [|t ts IHts]; auto.
+      cbn. erewrite IHts, instantiate_var_as_free_in_term; eauto.
+    - rewrite (IHF _ sigma); auto.
+    - rewrite (IHF1 _ sigma); auto. rewrite (IHF2 _ sigma); auto.
+    - rewrite (IHF1 _ sigma); auto. rewrite (IHF2 _ sigma); auto.
+    - rewrite (IHF1 _ sigma); auto. rewrite (IHF2 _ sigma); auto.
+    - rewrite (IHF1 _ sigma); auto. rewrite (IHF2 _ sigma); auto.
+    - destruct (x == s).
+      + (* in this case, [n + 1] does not appear in the FVs of F so the opening does nothing.
+           Also, it makes the translations equal (as [rho] and [sigma] are equal in all the other
+           values *) admit.
+      + rewrite (IHF (s :: rho) (s :: sigma) x (n + 1)).
+        * cbn. destruct (x == s); try congruence.
+          destruct (index_of x rho); cbn.
+          -- rewrite PeanoNat.Nat.add_1_r. injection ex => -> //.
+          -- inversion ex.
+        * intros; destruct m; cbn; auto.
+          apply erho. rewrite PeanoNat.Nat.add_1_r in H; lia.
+        * rewrite PeanoNat.Nat.add_1_r nth_error_cons_succ //.
+        * reflexivity.
+    - destruct (x == s).
+      + (* in this case, [n + 1] does not appear in the FVs of F so the opening does nothing.
+           Also, it makes the translations equal (as [rho] and [sigma] are equal in all the other
+           values *) admit.
+      + rewrite (IHF (s :: rho) (s :: sigma) x (n + 1)).
+        * cbn. destruct (x == s); try congruence.
+          destruct (index_of x rho); cbn.
+          -- rewrite PeanoNat.Nat.add_1_r. injection ex => -> //.
+          -- inversion ex.
+        * intros; destruct m; cbn; auto.
+          apply erho. rewrite PeanoNat.Nat.add_1_r in H; lia.
+        * rewrite PeanoNat.Nat.add_1_r nth_error_cons_succ //.
+        * reflexivity.
   Admitted.
 End ESyntaxTranslation.
 
@@ -236,6 +606,122 @@ Coercion translate_EForm : EForm >-> Form.
 
 (** ** 4. Correspondance of the syntax *)
 
+Section ValidityEquivalence.
+  Lemma interp_term_interp_eterm :
+    forall (M : Model string string) (t : ETerm) (rho : list M) (sigma : env M string),
+      interpret_term rho sigma [[ t ]] = interpret_eterm sigma t.
+  Proof.
+    intros ????. induction t using eterm_ind; cbn; auto.
+    rewrite map_map.
+    have Hmap : map (fun u => interpret_term rho sigma [[ u ]]) l = map (interpret_eterm sigma) l.
+    { induction l as [|x xs IHxs]; auto.
+      cbn. rewrite IHxs.
+      - now apply Forall_tail in H.
+      - apply Forall_In with (x := x) in H.
+        + rewrite H //.
+        + now right. }
+    rewrite Hmap //.
+  Qed.
+
+  Lemma interpret_eterm_map_interpret_term :
+    forall (M : Model string string) (l : list ETerm),
+      map (interpret_eterm (empty_env M string)) l =
+        map (fun u => interpret_term [] (empty_env M string) [[ u ]]) l.
+  Proof.
+    intros ??. induction l as [|x xs IHxs]; auto.
+    cbn; rewrite interp_term_interp_eterm IHxs //.
+  Qed.
+
+  Lemma is_valid_translation_is_valid_ :
+    forall (F : EForm) (M : Model string string),
+      ([[ M # [] # (empty_env M string) |- [[F]]]]) <->
+        (interpret_eform M (empty_env M string) F).
+  Proof.
+    intros F; induction F;
+      intros M; split; intros hvalid.
+    all: try (cbn in *; auto; fail).
+
+    (** Cases: pred *)
+    - cbn in *; rewrite map_map in hvalid; rewrite interpret_eterm_map_interpret_term //.
+    - cbn in *; rewrite map_map -interpret_eterm_map_interpret_term //.
+
+    (** Cases: neg *)
+    - cbn in *; intro hvalid'; apply hvalid. now rewrite IHF.
+    - cbn in *; intro hvalid'; apply hvalid. now rewrite -IHF.
+
+    (** Cases: or *)
+    - cbn in *; destruct hvalid as [hvalid1 | hvalid2].
+      + left; now rewrite -IHF1.
+      + right; now rewrite -IHF2.
+    - cbn in *; destruct hvalid as [hvalid1 | hvalid2].
+      + left; now rewrite IHF1.
+      + right; now rewrite IHF2.
+
+    (** Cases: and *)
+    - cbn in *; split.
+      + apply NNPP => hnf1. apply hvalid. left. intro hf1. apply hnf1.
+        rewrite -IHF1 //.
+      + apply NNPP => hnf2. apply hvalid. right. intro hf2. apply hnf2.
+        rewrite -IHF2 //.
+    - cbn in *; intros [hf1 | hf2].
+      + apply hf1. rewrite IHF1. apply hvalid.
+      + apply hf2. rewrite IHF2. apply hvalid.
+
+    (** Cases: imp *)
+    - cbn in *; intro hf1. destruct hvalid as [hnf1 | hf2].
+      + exfalso. apply hnf1. rewrite IHF1 //.
+      + rewrite -IHF2 //.
+    - cbn in *; apply NNPP => save. apply save. right.
+      rewrite IHF2. apply hvalid. apply NNPP => hnf1. apply save. left. rewrite IHF1 //.
+
+    (** Cases: equ *)
+    - cbn in *; split.
+      + intros hf1. apply NNPP => hnf2. apply hvalid. left. intros [hnf1 | hf2].
+        * apply hnf1. rewrite IHF1 //.
+        * apply hnf2. rewrite -IHF2 //.
+      + intros hf2. apply NNPP => hnf1. apply hvalid. right. intros [hnf2 | hf1].
+        * apply hnf2. rewrite IHF2 //.
+        * apply hnf1. rewrite -IHF1 //.
+    - cbn in *; intros [himp | himp]; apply himp;
+        rewrite IHF2 IHF1 hvalid; apply imply_to_or; tauto.
+
+    (** Cases: ex *)
+    - cbn in *.
+      apply NNPP => save. apply hvalid => x hF.
+      apply save. exists x.
+
+      (* TODO: show this: *)
+      have H : forall M x rho (F : Form) s,
+          [[ M # {{ x }} # rho |- F ]] =
+            [[ M # [] # (fun y => match s == y with
+                               | left _ => Some x
+                               | right _ => rho y
+                               end) |- (F{0 \to Free s}) ]].
+      { admit. }
+      rewrite (H _ _ _ _ s) in hF.
+      rewrite (instantiate_var_as_free_in_form _ _ []) in hF.
+      + cbn; destruct (s == s); auto. exfalso; now apply n.
+      + intros m contra; inversion contra.
+      + reflexivity.
+      + admit. (* TODO: generalize IHF and this is free *)
+  Admitted.
+
+  Lemma is_valid_translation_is_valid :
+    forall (F : EForm), \models (translate_EForm F) <-> is_evalid F.
+  Proof.
+    intros F; split; intros H M; specialize (H M);
+      now apply is_valid_translation_is_valid_.
+  Qed.
+
+  Lemma hasTableau_is_evalid :
+    forall (F : EForm) (sko : Skolemization) (sigma : Substitution string Term),
+      hasTableau sko {{ Neg [[ F ]] }} sigma -> is_evalid F.
+  Proof.
+    intros ??? htab. apply (hasTableau_sound sko [[ F ]] sigma) in htab.
+    now rewrite -is_valid_translation_is_valid.
+  Qed.
+End ValidityEquivalence.
+
 (** ** 5. Helper to transform substitution into internal substitution *)
 Section TranslateSubst.
   Fixpoint subst_translation (l : list (string * ETerm)) : string -> Term :=
@@ -248,29 +734,28 @@ Section TranslateSubst.
     end.
 
   Lemma eterm_translation_is_always_locally_closed :
-    forall (t : ETerm), @LocallyClosed _ Term _ [[ t ]].
+    forall (t : ETerm), @isLocallyClosed _ Term _ [[ t ]].
   Proof.
     intro t. induction t using eterm_ind.
-    - cbn; rewrite is_empty_spec //.
-    - induction l as [|x xs IHxs].
-      + cbn; rewrite is_empty_spec //.
-      + cbn. rewrite empty_unitl.
+    - unfold isLocallyClosed; cbn. apply empty_is_empty.
+    - induction l as [|x xs IHxs]; unfold isLocallyClosed; cbn.
+      + apply empty_is_empty.
+      + rewrite empty_unitl.
         have Hbv := Forall_In _ _ H x (ltac:(now right)).
         red in Hbv. unfold is_empty in Hbv; cbn in Hbv.
-        rewrite is_empty_spec in Hbv. rewrite Hbv.
-        cbn. apply IHxs, In_Forall=>u hu.
+        rewrite Hbv. apply IHxs, In_Forall=>u hu.
         apply Forall_In with (x := u) in H; auto.
         now left.
   Qed.
 
   Lemma locally_closed_subst_translation :
     forall (l : list (string * ETerm)) (x : string),
-      (forall (x : string) (t : ETerm), In (x, t) l -> @LocallyClosed _ Term _ [[ t ]]) ->
-      LocallyClosed (subst_translation l x).
+      (forall (x : string) (t : ETerm), In (x, t) l -> @isLocallyClosed _ Term _ [[ t ]]) ->
+      isLocallyClosed (subst_translation l x).
   Proof.
-    intros l x H. induction l as [|y ys IHys].
-    - cbn; rewrite is_empty_spec //.
-    - cbn. destruct (fst y == x).
+    intros l x H. induction l as [|y ys IHys]; unfold isLocallyClosed; cbn.
+    - apply empty_is_empty.
+    - destruct (fst y == x).
       + eapply (H (fst y)). right. now destruct y.
       + apply IHys. intros; apply (H x0).
         now left.
@@ -292,7 +777,7 @@ Section HasTableauLemmas.
 
   Lemma con_nth_in :
     forall (Gamma : Con) (i : nat) (F : Form),
-      con_nth Gamma i = Some F -> F \in Gamma.
+      nth_error Gamma i = Some F -> F \in Gamma.
   Proof using Type.
     intros ??? e. generalize dependent i. induction Gamma as [|x xs IHxs]; cbn in *;
       intros i e.
@@ -306,7 +791,7 @@ Section HasTableauLemmas.
 
   Lemma hasTableauBot :
     forall (Gamma : Con) (sigma : Substitution string Term) (S Sf : SetOfString) (i : nat),
-      con_nth Gamma i = Some [[ EBot ]] -> hasTableau_ sko Gamma S Sf sigma.
+      nth_error Gamma i = Some [[ EBot ]] -> hasTableau_ sko Gamma S Sf sigma.
   Proof using Type.
     intros ????? e. apply hasTableauBot.
     eapply con_nth_in; eauto.
@@ -314,7 +799,7 @@ Section HasTableauLemmas.
 
   Lemma hasTableauNegTop :
     forall (Gamma : Con) (sigma : Substitution string Term) (S Sf : SetOfString) (i : nat),
-      con_nth Gamma i = Some [[ ENeg ETop ]] -> hasTableau_ sko Gamma S Sf sigma.
+      nth_error Gamma i = Some [[ ENeg ETop ]] -> hasTableau_ sko Gamma S Sf sigma.
   Proof using Type.
     intros ????? e. eapply hasTableauNegNeg.
     - cbn in e. eapply con_nth_in; eauto.
@@ -323,7 +808,7 @@ Section HasTableauLemmas.
 
   Lemma hasTableauContr :
     forall (Gamma : Con) (sigma : Substitution string Term) (S Sf : SetOfString) (i j : nat) (F G : EForm),
-      con_nth Gamma i = Some [[ F ]] -> con_nth Gamma j = Some [[ G ]] ->
+      nth_error Gamma i = Some [[ F ]] -> nth_error Gamma j = Some [[ G ]] ->
       (etranslation_eform (ENeg F))@[sigma] = (etranslation_eform G)@[sigma] ->
       hasTableau_ sko Gamma S Sf sigma.
   Proof using Type.
@@ -336,7 +821,7 @@ Section HasTableauLemmas.
 
   Lemma hasTableauNegNeg :
     forall (Gamma : Con) (sigma : Substitution string Term) (S Sf : SetOfString) (i : nat) (F : EForm),
-      con_nth Gamma i = Some [[ ENeg (ENeg F) ]] ->
+      nth_error Gamma i = Some [[ ENeg (ENeg F) ]] ->
       hasTableau_ sko (Gamma ,, [[ F ]]) S Sf sigma ->
       hasTableau_ sko Gamma S Sf sigma.
   Proof using Type.
@@ -346,7 +831,7 @@ Section HasTableauLemmas.
 
   Lemma hasTableauAnd :
     forall (Gamma : Con) (sigma : Substitution string Term) (S Sf : SetOfString) (i : nat) (F G : EForm),
-      con_nth Gamma i = Some [[ EAnd F G ]] ->
+      nth_error Gamma i = Some [[ EAnd F G ]] ->
       hasTableau_ sko (Gamma ,, Neg (Neg [[ F ]]) ,, Neg (Neg [[ G ]]) ,, [[ F ]] ,, [[ G ]]) S Sf sigma ->
       hasTableau_ sko Gamma S Sf sigma.
   Proof using Type.
@@ -365,7 +850,7 @@ Section HasTableauLemmas.
 
   Lemma hasTableauNegOr :
     forall (Gamma : Con) (sigma : Substitution string Term) (S Sf : SetOfString) (i : nat) (F G : EForm),
-      con_nth Gamma i = Some [[ ENeg (EOr F G) ]] ->
+      nth_error Gamma i = Some [[ ENeg (EOr F G) ]] ->
       hasTableau_ sko (Gamma ,, Neg [[ F ]] ,, Neg [[ G ]]) S Sf sigma ->
       hasTableau_ sko Gamma S Sf sigma.
   Proof using Type.
@@ -376,7 +861,7 @@ Section HasTableauLemmas.
 
   Lemma hasTableauNegImp :
     forall (Gamma : Con) (sigma : Substitution string Term) (S Sf : SetOfString) (i : nat) (F G : EForm),
-      con_nth Gamma i = Some [[ ENeg (EImp F G) ]] ->
+      nth_error Gamma i = Some [[ ENeg (EImp F G) ]] ->
       hasTableau_ sko (Gamma ,, Neg (Neg [[ F ]]) ,, Neg [[ G ]] ,, [[ F ]]) S Sf sigma ->
       hasTableau_ sko Gamma S Sf sigma.
   Proof using Type.
@@ -391,7 +876,7 @@ Section HasTableauLemmas.
 
   Lemma hasTableauOr :
     forall (Gamma : Con) (sigma : Substitution string Term) (S1 S2 Sf1 Sf2 : SetOfString) (i : nat) (F G : EForm),
-      con_nth Gamma i = Some [[ EOr F G ]] ->
+      nth_error Gamma i = Some [[ EOr F G ]] ->
       hasTableau_ sko (Gamma ,, [[ F ]]) S1 Sf1 sigma ->
       hasTableau_ sko (Gamma ,, [[ G ]]) S2 Sf2 sigma -> disjoint S1 S2 -> disjoint Sf1 Sf2 ->
       hasTableau_ sko Gamma (S1 \union S2) (Sf1 \union Sf2) sigma.
@@ -403,7 +888,7 @@ Section HasTableauLemmas.
 
   Lemma hasTableauImp :
     forall (Gamma : Con) (sigma : Substitution string Term) (S1 S2 Sf1 Sf2 : SetOfString) (i : nat) (F G : EForm),
-      con_nth Gamma i = Some [[ EImp F G ]] ->
+      nth_error Gamma i = Some [[ EImp F G ]] ->
       hasTableau_ sko (Gamma ,, [[ ENeg F ]]) S1 Sf1 sigma ->
       hasTableau_ sko (Gamma ,, [[ G ]]) S2 Sf2 sigma -> disjoint S1 S2 -> disjoint Sf1 Sf2 ->
       hasTableau_ sko Gamma (S1 \union S2) (Sf1 \union Sf2) sigma.
@@ -415,7 +900,7 @@ Section HasTableauLemmas.
 
   Lemma hasTableauNegAnd :
     forall (Gamma : Con) (sigma : Substitution string Term) (S1 S2 Sf1 Sf2 : SetOfString) (i : nat) (F G : EForm),
-      con_nth Gamma i = Some [[ ENeg (EAnd F G) ]] ->
+      nth_error Gamma i = Some [[ ENeg (EAnd F G) ]] ->
       hasTableau_ sko (Gamma ,, (Or [[ ENeg F ]] [[ ENeg G ]]) ,, [[ ENeg F ]]) S1 Sf1 sigma ->
       hasTableau_ sko (Gamma ,, (Or [[ ENeg F ]] [[ ENeg G ]]) ,, [[ ENeg G ]]) S2 Sf2 sigma ->
       disjoint S1 S2 -> disjoint Sf1 Sf2 ->
@@ -432,7 +917,7 @@ Section HasTableauLemmas.
 
   Lemma hasTableauEqu :
     forall (Gamma : Con) (sigma : Substitution string Term) (S1 S2 Sf1 Sf2 : SetOfString) (i : nat) (F G : EForm),
-      con_nth Gamma i = Some [[ (EEqu F G) ]] ->
+      nth_error Gamma i = Some [[ (EEqu F G) ]] ->
       hasTableau_ sko (Gamma ,, Neg [[ ENeg (EImp F G) ]] ,, Neg [[ ENeg (EImp G F) ]] ,,
                          [[ EImp F G ]] ,, [[ EImp G F ]] ,, [[ ENeg F ]] ,, [[ ENeg G ]])
         S1 Sf1 sigma ->
@@ -459,8 +944,8 @@ Section HasTableauLemmas.
           -- exact (ENeg F).
           -- exact G.
           -- now cbn.
-          -- replace S1 with (S1 \union (empty_set string)).
-             replace Sf1 with (Sf1 \union (empty_set string)).
+          -- replace S1 with (S1 \union empty_set).
+             replace Sf1 with (Sf1 \union empty_set).
              2, 3: apply empty_unitr.
              unshelve eapply hasTableauOr.
              ++ exact 1.
@@ -478,8 +963,8 @@ Section HasTableauLemmas.
                 ** reflexivity.
              ++ apply empty_disjointr.
              ++ apply empty_disjointr.
-          -- replace S2 with ((empty_set string) \union S2).
-             replace Sf2 with ((empty_set string) \union Sf2).
+          -- replace S2 with (empty_set \union S2).
+             replace Sf2 with (empty_set \union Sf2).
              2,3 : apply empty_unitl.
              unshelve eapply hasTableauOr.
              ++ exact 1.
@@ -503,7 +988,7 @@ Section HasTableauLemmas.
 
   Lemma hasTableauNegEqu :
     forall (Gamma : Con) (sigma : Substitution string Term) (S1 S2 Sf1 Sf2 : SetOfString) (i : nat) (F G : EForm),
-      con_nth Gamma i = Some [[ ENeg (EEqu F G) ]] ->
+      nth_error Gamma i = Some [[ ENeg (EEqu F G) ]] ->
       hasTableau_ sko (Gamma ,, [[ EOr (ENeg (EImp F G)) (ENeg (EImp G F)) ]] ,, [[ ENeg (EImp F G) ]]
                          ,, [[ ENeg (ENeg F) ]] ,, [[ ENeg G ]] ,, [[ F ]]) S1 Sf1 sigma ->
       hasTableau_ sko (Gamma ,, [[ EOr (ENeg (EImp F G)) (ENeg (EImp G F)) ]] ,, [[ ENeg (EImp G F) ]]
@@ -533,7 +1018,7 @@ Section HasTableauLemmas.
   Lemma hasTableauAll :
     forall (Gamma : Con) (sigma : Substitution string Term) (S Sf : SetOfString) (i : nat) (F : EForm)
       (x : string) (y : string),
-      con_nth Gamma i = Some [[ EAll x F ]] -> isFresh y S ->
+      nth_error Gamma i = Some [[ EAll x F ]] -> isFresh y S ->
       hasTableau_ sko (Gamma ,, [[ instantiate_eform x (EVar y) F ]]) S Sf sigma ->
       hasTableau_ sko Gamma (add y S) Sf sigma.
   Proof.
@@ -548,7 +1033,7 @@ Section HasTableauLemmas.
     forall (Gamma : Con) (sigma : Substitution string Term) (S Sf : SetOfString) (i : nat) (F : EForm)
       (x : string) (t : ETerm) (f : string)
       (hsko : is_sko [[ t ]] (Neg (translate_EForm_ [x] F)) (fv Gamma) Sf),
-      con_nth Gamma i = Some [[ ENeg (EAll x F) ]] -> symbol sko [[ t ]] hsko = f ->
+      nth_error Gamma i = Some [[ ENeg (EAll x F) ]] -> symbol sko [[ t ]] hsko = f ->
       hasTableau_ sko (Gamma ,, [[ instantiate_eform x t (ENeg F) ]]) S Sf sigma ->
       hasTableau_ sko Gamma S (add f Sf) sigma.
   Proof.
@@ -562,7 +1047,7 @@ Section HasTableauLemmas.
     forall (Gamma : Con) (sigma : Substitution string Term) (S Sf : SetOfString) (i : nat) (F : EForm)
       (x : string) (t : ETerm) (f : string)
       (hsko : is_sko [[ t ]] (Neg (translate_EForm_ [x] (ENeg F))) (fv Gamma) Sf),
-      con_nth Gamma i = Some [[ EEx x F ]] -> symbol sko [[ t ]] hsko = f ->
+      nth_error Gamma i = Some [[ EEx x F ]] -> symbol sko [[ t ]] hsko = f ->
       hasTableau_ sko (Gamma ,, [[ ENeg (ENeg (instantiate_eform x t F)) ]] ,,
                          [[ instantiate_eform x t F ]]) S Sf sigma ->
       hasTableau_ sko Gamma S (add f Sf) sigma.
@@ -583,7 +1068,7 @@ Section HasTableauLemmas.
   Lemma hasTableauNegEx :
     forall (Gamma : Con) (sigma : Substitution string Term) (S Sf : SetOfString) (i : nat) (F : EForm)
       (x : string) (y : string),
-      con_nth Gamma i = Some [[ ENeg (EEx x F) ]] -> isFresh y S ->
+      nth_error Gamma i = Some [[ ENeg (EEx x F) ]] -> isFresh y S ->
       hasTableau_ sko (Gamma ,, [[EAll x (ENeg F)]] ,, [[ instantiate_eform x (EVar y) (ENeg F) ]])
         S Sf sigma -> hasTableau_ sko Gamma (add y S) Sf sigma.
   Proof using Type.
