theories/Proofs.v
@@ -5,62 +5,60 @@ From Tableaux Require Import Skolemization.
 From Tableaux Require Import Syntax.
 
 Section TableauxProofs.
-  Context `{set_nat : set nat} {pred func var : Atom} {con : Con_ pred func var}
-    (sko : Skolemization_ pred func var).
+  Context `{set_nat : set nat} {pred func var : Atom} (sko : Skolemization_ pred func var).
 
   Let set_var := set_atom var.
   Let set_func := set_atom func.
 
   Inductive hasTableau_
-    : con -> set_var -> set_func -> Substitution var (Term_ func var) -> Prop :=
+    : Con_ pred func var -> set_var -> set_func -> Substitution var (Term_ func var) -> Prop :=
 
   (** Axioms *)
   | hasTableauBot :
-    forall (Gamma : con) (S : set_var) (Sf : set_func) (sigma : Substitution var (Term_ func var)),
+    forall (Gamma : Con_ pred func var) (S : set_var) (Sf : set_func) (sigma : Substitution var (Term_ func var)),
       (Bot \in Gamma) -> hasTableau_ Gamma S Sf sigma
   | hasTableauContr :
-    forall (Gamma : con) (S : set_var) (Sf : set_func) (sigma : Substitution var (Term_ func var))
+    forall (Gamma : Con_ pred func var) (S : set_var) (Sf : set_func) (sigma : Substitution var (Term_ func var))
       (P P' : Form_ pred func var), (P \in Gamma) -> (P' \in Gamma) -> Neg P@[sigma] = P'@[sigma] -> hasTableau_ Gamma S Sf sigma
 
   (** Alpha rules *)
   | hasTableauNegNeg :
-    forall (Gamma : con) (S : set_var) (Sf : set_func) (sigma : Substitution var (Term_ func var))
+    forall (Gamma : Con_ pred func var) (S : set_var) (Sf : set_func) (sigma : Substitution var (Term_ func var))
       (F : Form_ pred func var), Neg (Neg F) \in Gamma -> hasTableau_ (Gamma ,, F) S Sf sigma -> hasTableau_ Gamma S Sf sigma
   | hasTableauNegOr :
-    forall (Gamma : con) (S : set_var) (Sf : set_func) (sigma : Substitution var (Term_ func var))
+    forall (Gamma : Con_ pred func var) (S : set_var) (Sf : set_func) (sigma : Substitution var (Term_ func var))
       (F1 F2 : Form_ pred func var),
       Neg (Or F1 F2) \in Gamma -> hasTableau_ (Gamma ,, Neg F1 ,, Neg F2) S Sf sigma -> hasTableau_ Gamma S Sf sigma
 
   (** Beta rule *)
   | hasTableauOr :
-    forall (Gamma : con) (S1 S2 : set_var) (Sf1 Sf2 : set_func) (sigma : Substitution var (Term_ func var))
+    forall (Gamma : Con_ pred func var) (S1 S2 : set_var) (Sf1 Sf2 : set_func) (sigma : Substitution var (Term_ func var))
       (F1 F2 : Form_ pred func var),
       (Or F1 F2) \in Gamma -> hasTableau_ (Gamma ,, F1) S1 Sf1 sigma -> hasTableau_ (Gamma ,, F2) S2 Sf2 sigma ->
       disjoint S1 S2 -> disjoint Sf1 Sf2 -> hasTableau_ Gamma (S1 \union S2) (Sf1 \union Sf2) sigma
 
   (** Gamma rule *)
   | hasTableauAll :
-    forall (Gamma : con) (S : set_var) (Sf : set_func) (sigma : Substitution var (Term_ func var))
+    forall (Gamma : Con_ pred func var) (S : set_var) (Sf : set_func) (sigma : Substitution var (Term_ func var))
       (x : var) (F : Form_ pred func var),
       (All F) \in Gamma -> isFresh x S -> hasTableau_ (Gamma ,, F{0 \to Free x}) S Sf sigma ->
       hasTableau_ Gamma (add x S) Sf sigma
 
    (** Delta rule *)
   | hasTableauNegAll :
-    forall (Gamma : con) (S : set_var) (Sf : set_func) (sigma : Substitution var (Term_ func var))
+    forall (Gamma : Con_ pred func var) (S : set_var) (Sf : set_func) (sigma : Substitution var (Term_ func var))
       (F : Form_ pred func var) (t : Term_ func var) (Hsko : is_sko t (Neg F) (fv Gamma) Sf),
       (Neg (All F)) \in Gamma -> hasTableau_ (Gamma ,, Neg F{0 \to t}) S Sf sigma ->
       hasTableau_ Gamma S (add (symbol sko t Hsko) Sf) sigma.
 
-  Definition hasTableau (Gamma : con) (sigma : Substitution var (Term_ func var)) : Prop :=
+  Definition hasTableau (Gamma : Con_ pred func var) (sigma : Substitution var (Term_ func var)) : Prop :=
     exists (S : set_var) (Sf : set_func), hasTableau_ Gamma S Sf sigma.
 End TableauxProofs.
 
 (* TODO: structural lemmas, e.g., strengthening, exchange law, (need something else?) *)
 
 Section TableauxSoundness.
-  Context `{set_nat : set nat} {pred func var : Atom} {con : Con_ pred func var}
-    (sko : Skolemization_ pred func var).
+  Context `{set_nat : set nat} {pred func var : Atom} (sko : Skolemization_ pred func var).
 
   Theorem hasTableau_sound :
     forall (F : Form_ pred func var) (sigma : Substitution var (Term_ func var)),
