theories/Syntax.v
@@ -1,10 +1,8 @@
 (** * Syntax: definition of a locally-nameless first-order logic syntax. *)
 
-From Tableaux Require Export Prelude.
+From Tableaux Require Export Prelude.All.
 
 From Stdlib Require Import Structures.Orders.
-
-Import ListNotations.
 
 (** ** First-order logic terms *)
 
@@ -14,7 +12,6 @@ Inductive Term_ {func var : Atom} : Type :=
 | Fun   : func -> list Term_ -> Term_.
 
 Arguments Term_ : clear implicits.
-Definition Term := Term_ string string.
 
 (** *** Better induction principles for terms *)
 Section TermInd.
@@ -94,194 +91,6 @@ Section DecEqTerms.
   Qed.
 End DecEqTerms.
 
-(** Set of [Term]s. *)
-Module OrderedTerm <: OrderedType.
-  Definition t := Term.
-  Definition eq := @eq Term.
-  Definition eq_equiv := @eq_equivalence Term.
-
-  Inductive lt_list {A : Type} {lt : A -> A -> Prop} : list A -> list A -> Prop :=
-  | lt_head : forall (t u : A) (l l' : list A), lt t u -> lt_list (t :: l) (u :: l')
-  | lt_cons : forall (t : A) (l l' : list A), lt_list l l' -> lt_list (t :: l) (t :: l').
-  Arguments lt_list {_} _ _ _.
-
-  Lemma lt_list_irrefl :
-    forall {A : Type} {lt : A -> A -> Prop} (l : list A),
-      (forall t, In t l -> lt t t -> False) -> lt_list lt l l -> False.
-  Proof.
-    intros A lt l hirrefl hlt.
-    have H0 : exists l', lt_list lt l l' /\ l = l' by exists l.
-    destruct H0 as (l' & H' & e); induction H'.
-    + injection e => e0 e1; subst. unshelve eapply hirrefl.
-      * exact u.
-      * now right.
-      * assumption.
-    + injection e => e0; subst. apply IHH'; auto.
-      intros; eapply hirrefl; eauto. now left.
-  Qed.
-
-  Fixpoint compare_list {A : Type} (cmp : A -> A -> comparison) (l l' : list A) : comparison :=
-    match l, l' with
-    | [], [] => Eq
-    | [], _  => Lt
-    | _ , [] => Gt
-    | x :: xs, y :: ys =>
-        match cmp x y with
-        | Eq => compare_list cmp xs ys
-        | _ as v => v
-        end
-    end.
-
-  Inductive lt_ : Term -> Term -> Prop :=
-  | termLtBoundBound : forall (n m : nat), n < m -> lt_ (Bound n) (Bound m)
-  | termLtBoundFree  : forall (n : nat) (x : string), lt_ (Bound n) (Free x)
-  | termLtBoundFun   : forall (n : nat) (f : string) (l : list Term), lt_ (Bound n) (Fun f l)
-  | termLtFreeFree   : forall (x y : string), OrderedString.lt x y -> lt_ (Free x) (Free y)
-  | termLtFreeFun    : forall (x : string) (f : string) (l : list Term), lt_ (Free x) (Fun f l)
-  | termLtFunFun1    : forall (f f' : string) (l l' : list Term),
-      OrderedString.lt f f' -> lt_ (Fun f l) (Fun f' l')
-  | termLtFunFun2    : forall (f : string) (l l' : list Term),
-      lt_list lt_ l l' -> lt_ (Fun f l) (Fun f l').
-
-  (* Definition lt_ind' (P : Term -> Term -> Prop) (f : forall n m : nat, n < m -> P (Bound n) (Bound m)) *)
-  (*   (f0 : forall (n : nat) (x : string), P (Bound n) (Free x)) *)
-  (*   (f1 : forall (n : nat) (f1 : string) (l : list Term), P (Bound n) (Fun f1 l)) *)
-  (*   (f2 : forall x y : string, OrderedString.lt x y -> P (Free x) (Free y)) *)
-  (*   (f3 : forall (x f3 : string) (l : list Term), P (Free x) (Fun f3 l)) *)
-  (*   (f4 : forall (f4 f' : string) (l l' : list Term), OrderedString.lt f4 f' -> P (Fun f4 l) (Fun f' l')) *)
-  (*   (f5 : forall (f5 : string) (l l' : list Term), *)
-  (*       (forall i t u, nth_error l i = Some t -> nth_error l' i = Some u -> lt t u -> P t u) -> *)
-  (*       lt_list lt l l' -> P (Fun f5 l) (Fun f5 l')) *)
-  (*    : forall (t t0 : Term), lt t t0 -> P t t0. *)
-  (* Proof. *)
-  (*   refine (fix F (t t0 : Term) (h : lt t t0) : P t t0 := *)
-  (*             let fix F_list (l l' : list Term) (h0 : lt_list lt l l') : *)
-  (*               (forall i t u, nth_error l i = Some t -> nth_error l' i = Some u -> lt t u -> P t u) := _ *)
-  (*             in *)
-  (*             match h in (lt t1 t2) return (P t1 t2) with *)
-  (*             | termLtBoundBound n m x => f n m x *)
-  (*             | termLtBoundFree n x => f0 n x *)
-  (*             | termLtBoundFun n f6 l0 => f1 n f6 l0 *)
-  (*             | termLtFreeFree x y x0 => f2 x y x0 *)
-  (*             | termLtFreeFun x f6 l0 => f3 x f6 l0 *)
-  (*             | termLtFunFun1 f6 f' l0 l' x => f4 f6 f' l0 l' x *)
-  (*             | termLtFunFun2 f6 l0 l' x => f5 f6 l0 l' (F_list l0 l' x) x *)
-  (*             end). *)
-  (*   intros. destruct h0. *)
-  (*   - now apply F. *)
-  (*   - destruct i; cbn in *. *)
-  (*     + now apply F. *)
-  (*     + eapply F_list; eauto. *)
-  (* Defined. *)
-
-  Definition lt := lt_.
-
-  Lemma lt_strorder : StrictOrder lt.
-  Proof. Admitted.
-    (* split. *)
-    (* - intros t H. *)
-    (*   have H0 : exists u, lt t u /\ t = u by exists t. *)
-    (*   destruct H0 as (u & H' & e); induction H'; *)
-    (*     try (inversion e; fail). *)
-    (*   + injection e => e'. rewrite e' in H0. *)
-    (*     now apply StrictOrder_Irreflexive in H0. *)
-    (*   + injection e => e'. rewrite e' in H0. *)
-    (*     now apply StrictOrder_Irreflexive in H0. *)
-    (*   + injection e => _ e'. rewrite e' in H0. *)
-    (*     now apply StrictOrder_Irreflexive in H0. *)
-    (*   + injection e => e'; subst. eapply lt_list_irrefl. *)
-    (*     2: exact H0. *)
-        
-        
-    (*     intros. *)
-    (*   apply H. intros l hlt. *)
-    (*   have H0 : exists l', lt_list l l' /\ l = l' by exists l. *)
-    (*   destruct H0 as (l' & H' & e); induction H'. *)
-    (*   + injection e => e0 e1; subst. *)
-    (*     have contra : (lt u u -> False). *)
-    (*     { apply H. intro. intro. *)
-    (*     injection e' => _ e0. subst. apply IHH'; auto. *)
-    (* - intros t u v htu huv. *)
-    (*   have H0 : exists u', lt u' v /\ u = u' by exists u. *)
-    (*   destruct H0 as (u' & H' & e). clear huv. induction htu; destruct H'. *)
-    (*   (** trivial cases *) *)
-    (*   all: try now constructor. *)
-    (*   (** inconsistency in the equality *) *)
-    (*   all: try (inversion e; fail). *)
-    (*   + constructor. eapply StrictOrder_Transitive; eauto. *)
-    (*     injection e => e'; now subst. *)
-    (*   + constructor. eapply StrictOrder_Transitive; eauto. *)
-    (*     injection e => e'; now subst. *)
-    (*   + injection e => e' e''; subst. constructor. *)
-    (*     eapply StrictOrder_Transitive; eauto. *)
-    (*   + injection e => e' e''; subst; now constructor. *)
-    (*   + injection e => e' e''; subst; now constructor. *)
-    (*   + injection e => e' e''. rewrite e''. *)
-    (*     have H : lt t0 u0. *)
-    (*     {  *)
-    (*     eapply termLtFunFun2. *)
-
-  Lemma lt_compat : Proper (Logic.eq ==> Logic.eq ==> iff) lt.
-  Proof.
-    intros t u e t' u' e'. split.
-    + intros; now subst.
-    + intros; now subst.
-  Qed.
-
-  Fixpoint compare (t u : Term) : comparison :=
-    match t, u with
-    | Bound n, Bound m => OrderedNat.compare n m
-    | Bound _, Free  _ => Lt
-    | Bound _, Fun _ _ => Lt
-    | Free _ , Bound _ => Gt
-    | Free x , Free y  => OrderedString.compare x y
-    | Free _ , Fun _ _ => Lt
-    | Fun _ _, Bound _ => Gt
-    | Fun _ _, Free _ => Gt
-    | Fun x xs, Fun y ys =>
-        match OrderedString.compare x y with
-        | Eq => compare_list compare xs ys
-        | _ as v => v
-        end
-    end.
-
-  Lemma compare_spec :
-    forall t u : Term, CompareSpec (t = u) (lt t u) (lt u t) (compare t u).
-  Proof.
-    intros t u; destruct t, u; cbn.
-    - destruct (OrderedNat.compare n n0) eqn:e.
-      + constructor.
-        apply PeanoNat.Nat.compare_eq in e; now subst.
-      + constructor.
-        apply PeanoNat.Nat.compare_lt_iff in e. now constructor.
-      + constructor.
-        apply PeanoNat.Nat.compare_gt_iff in e. now constructor.
-    - do 2 constructor.
-    - do 2 constructor.
-    - do 2 constructor.
-    - have H := (OrderedString.compare_spec a a0); destruct H.
-      + constructor. now rewrite H.
-      + now do 2 constructor.
-      + now do 2 constructor.
-    - do 2 constructor.
-    - do 2 constructor.
-    - do 2 constructor.
-    - have H := (OrderedString.compare_spec a a0); destruct H.
-      + generalize dependent l0. induction l; destruct l0.
-        * constructor. now rewrite H.
-        * constructor. admit.
-        * constructor. admit.
-        * admit.
-      + now do 2 constructor.
-      + now do 2 constructor.
-  Admitted.
-
-  Definition eq_dec := @eqDec Term _.
-End OrderedTerm.
-
-Module SetOfTerm_ := SetFromOrdered OrderedTerm.
-Canonical Structure SetOfTerm := SetOfTerm_.set_of_ordered.
-
 (** *** Opening and substitution for terms *)
 Section OpeningSubstTerms.
   Context {func var : Atom} `{set_nat : set nat}.
@@ -303,8 +112,8 @@ Section OpeningSubstTerms.
     fix F (t : Term_ func var) : set_nat :=
       match t with
       | Bound m => singleton m
-      | Free  _ => empty_set nat
-      | Fun _ l => fold_left (fun s t => s \union (F t)) l (empty_set nat)
+      | Free  _ => empty_set
+      | Fun _ l => fold_left (fun s t => s \union (F t)) l empty_set
       end.
 
   #[global] Instance subst_term : Subst (Term_ func var) (Term_ func var) :=
@@ -326,9 +135,9 @@ Section FVTerms.
   #[global] Instance fv_term : FV (Term_ func var) :=
     fix F (t : Term_ func var) : set_var :=
       match t with
-      | Bound _ => empty_set var
+      | Bound _ => empty_set
       | Free  x => singleton x
-      | Fun f l => fold_left (fun s t => s \union (F t)) l (empty_set var)
+      | Fun f l => fold_left (fun s t => s \union (F t)) l empty_set
       end.
 End FVTerms.
 
@@ -341,7 +150,6 @@ Inductive Form_ {pred func var : Atom} : Type :=
 | All  : Form_ -> Form_.
 
 Arguments Form_ : clear implicits.
-Definition Form := Form_ string string string.
 
 (** *** Decidable equality for formulas *)
 Section DecEqForms.
@@ -379,16 +187,17 @@ Section OpeningSubstForms.
   Context {pred func var : Atom} `{set_nat : set nat}.
   Existing Instance bv_term.
 
+  Fixpoint opening_form_ (n : nat) (u : Term_ func var) (F : Form_ pred func var) :=
+    match F with
+    | Bot => Bot
+    | Pred p l => Pred p (map (fun t => t{n \to u}) l)
+    | Neg  F'  => Neg (opening_form_ n u F')
+    | Or F1 F2 => Or (opening_form_ n u F1) (opening_form_ n u F2)
+    | All  F'  => All (opening_form_ (n+1) u F')
+    end.
+
   #[global] Instance opening_form : Opening (Term_ func var) (Form_ pred func var) :=
-    fun n u =>
-      (fix rec (n : nat) (F : Form_ pred func var) : Form_ pred func var :=
-         match F with
-         | Bot      => Bot
-         | Pred p l => Pred p (map (fun t => t{n \to u}) l)
-         | Neg  F'  => Neg (rec n F')
-         | Or F1 F2 => Or (rec n F1) (rec n F2)
-         | All  F'  => All (rec (n+1) F')
-         end) n.
+    opening_form_.
 
   #[global] Instance subst_form : Subst (Form_ pred func var) (Term_ func var) :=
     fun F sigma =>
@@ -411,8 +220,8 @@ Section FVForms.
   #[global] Instance fv_form : FV (Form_ pred func var) :=
     fix rec (F : Form_ pred func var) : set_var :=
       match F with
-      | Bot      => empty_set var
-      | Pred f l => fold_left (fun s t => s \union (fv t)) l (empty_set var)
+      | Bot      => empty_set
+      | Pred f l => fold_left (fun s t => s \union (fv t)) l empty_set
       | Neg F'   => rec F'
       | Or F1 F2 => (rec F1) \union (rec F2)
       | All F'   => rec F'
@@ -420,54 +229,223 @@ Section FVForms.
 End FVForms.
 
 (** ** Contexts *)
+Definition Con_ (pred func var : Atom) := list (Form_ pred func var).
 
-Class Con_ {pred func var : Atom} :=
-  { car :> Type
-  ; empty_con : car
-  ; extend : car -> Form_ pred func var -> car
-  ; in_ctx : Form_ pred func var -> car -> Type
-  ; con_nth : car -> nat -> option (Form_ pred func var)
-  ; con_ind : forall (P : car -> Type),
-      P empty_con ->
-      (forall (F : Form_ pred func var) (Gamma : car), P Gamma -> P (extend Gamma F)) ->
-      forall (Gamma : car), P Gamma}.
-Arguments empty_con {_ _ _ _}.
-Arguments extend {_ _ _ _} _ _.
-Arguments in_ctx {_ _ _ _} _ _.
-Arguments con_nth {_ _ _ _} _ _.
-Arguments Con_ : clear implicits.
+Notation "Gamma ,, A" := (A :: Gamma) (at level 20).
+Notation "A \in Gamma" := (In A Gamma) (at level 30).
 
-Notation "Gamma ,, A" := (extend Gamma A) (at level 20).
-Notation "A \in Gamma" := (in_ctx A Gamma) (at level 30).
-
-Canonical Structure Con : Con_ string string string :=
-  {| car := list Form
-  ;  empty_con := []
-  ;  extend := fun Gamma A => A :: Gamma
-  ;  in_ctx := In
-  ;  con_nth := @nth_error Form
-  ;  con_ind := @list_rect Form |}.
-Arguments Con : clear implicits.
-
-Notation "{{ F }}" := (empty_con ,, F).
+Notation "{{ F }}" := ([] ,, F).
 
 Section FVCon.
-  Context {pred func var : Atom} {con : Con_ pred func var}.
+  Context {pred func var : Atom}.
 
   Let set_var := set_atom var.
 
-  #[global] Instance fv_con : FV con.
-  Proof.
-    refine (con_ind (fun _ => set_var) _ _).
-    - exact (empty_set var).
-    - intros F Gamma s. exact (fv F \union s).
-  Defined.
+  #[global] Instance fv_con : FV (Con_ pred func var) :=
+    fix F (Gamma : Con_ pred func var) : set_var :=
+      match Gamma with
+      | [] => empty_set
+      | G :: Gamma => fv G \union (F Gamma)
+      end.
 End FVCon.
 
 (** ** Utils functions *)
-
 Definition get_symbol {func var : Atom} (t : Term_ func var) : option func :=
   match t with
   | Bound _ | Free _ => None
   | Fun f _ => Some f
   end.
+
+(** ** Concrete instances *)
+Module ConcreteSyntaxInstances.
+  Export AtomComputationalInstances.
+
+  Definition Term := Term_ string string.
+  Definition Form := Form_ string string string.
+  Definition Con := Con_ string string string.
+
+  (** *** Set of [Term]s. *)
+  Module OrderedTerm <: SimpleOrderedType.
+    Definition t := Term.
+
+    Inductive lt_list {A : Type} {lt : A -> A -> Prop} : list A -> list A -> Prop :=
+    | lt_head : forall (t u : A) (l l' : list A), lt t u -> lt_list (t :: l) (u :: l')
+    | lt_cons : forall (t : A) (l l' : list A), lt_list l l' -> lt_list (t :: l) (t :: l').
+    Arguments lt_list {_} _ _ _.
+
+    Lemma lt_list_irrefl :
+      forall {A : Type} {lt : A -> A -> Prop} (l : list A),
+        (forall t, In t l -> lt t t -> False) -> lt_list lt l l -> False.
+    Proof.
+      intros A lt l hirrefl hlt.
+      have H0 : exists l', lt_list lt l l' /\ l = l' by exists l.
+      destruct H0 as (l' & H' & e); induction H'.
+      - injection e => e0 e1; subst. unshelve eapply hirrefl.
+        + exact u.
+        + now right.
+        + assumption.
+      - injection e => e0; subst. apply IHH'; auto.
+        intros; eapply hirrefl; eauto. now left.
+    Qed.
+
+    Fixpoint compare_list {A : Type} (cmp : A -> A -> comparison) (l l' : list A) : comparison :=
+      match l, l' with
+      | [], [] => Eq
+      | [], _  => Lt
+      | _ , [] => Gt
+      | x :: xs, y :: ys =>
+          match cmp x y with
+          | Eq => compare_list cmp xs ys
+          | _ as v => v
+          end
+      end.
+
+    Inductive lt_ : Term -> Term -> Prop :=
+    | termLtBoundBound : forall (n m : nat), n < m -> lt_ (Bound n) (Bound m)
+    | termLtBoundFree  : forall (n : nat) (x : string), lt_ (Bound n) (Free x)
+    | termLtBoundFun   : forall (n : nat) (f : string) (l : list Term), lt_ (Bound n) (Fun f l)
+    | termLtFreeFree   : forall (x y : string), OrderedString.lt x y -> lt_ (Free x) (Free y)
+    | termLtFreeFun    : forall (x : string) (f : string) (l : list Term), lt_ (Free x) (Fun f l)
+    | termLtFunFun1    : forall (f f' : string) (l l' : list Term),
+        OrderedString.lt f f' -> lt_ (Fun f l) (Fun f' l')
+    | termLtFunFun2    : forall (f : string) (l l' : list Term),
+        lt_list lt_ l l' -> lt_ (Fun f l) (Fun f l').
+
+    (* Definition lt_ind' (P : Term -> Term -> Prop) (f : forall n m : nat, n < m -> P (Bound n) (Bound m)) *)
+    (*   (f0 : forall (n : nat) (x : string), P (Bound n) (Free x)) *)
+    (*   (f1 : forall (n : nat) (f1 : string) (l : list Term), P (Bound n) (Fun f1 l)) *)
+    (*   (f2 : forall x y : string, OrderedString.lt x y -> P (Free x) (Free y)) *)
+    (*   (f3 : forall (x f3 : string) (l : list Term), P (Free x) (Fun f3 l)) *)
+    (*   (f4 : forall (f4 f' : string) (l l' : list Term), OrderedString.lt f4 f' -> P (Fun f4 l) (Fun f' l')) *)
+    (*   (f5 : forall (f5 : string) (l l' : list Term), *)
+    (*       (forall i t u, nth_error l i = Some t -> nth_error l' i = Some u -> lt t u -> P t u) -> *)
+    (*       lt_list lt l l' -> P (Fun f5 l) (Fun f5 l')) *)
+    (*    : forall (t t0 : Term), lt t t0 -> P t t0. *)
+    (* Proof. *)
+    (*   refine (fix F (t t0 : Term) (h : lt t t0) : P t t0 := *)
+    (*             let fix F_list (l l' : list Term) (h0 : lt_list lt l l') : *)
+    (*               (forall i t u, nth_error l i = Some t -> nth_error l' i = Some u -> lt t u -> P t u) := _ *)
+    (*             in *)
+    (*             match h in (lt t1 t2) return (P t1 t2) with *)
+    (*             | termLtBoundBound n m x => f n m x *)
+    (*             | termLtBoundFree n x => f0 n x *)
+    (*             | termLtBoundFun n f6 l0 => f1 n f6 l0 *)
+    (*             | termLtFreeFree x y x0 => f2 x y x0 *)
+    (*             | termLtFreeFun x f6 l0 => f3 x f6 l0 *)
+    (*             | termLtFunFun1 f6 f' l0 l' x => f4 f6 f' l0 l' x *)
+    (*             | termLtFunFun2 f6 l0 l' x => f5 f6 l0 l' (F_list l0 l' x) x *)
+    (*             end). *)
+    (*   intros. destruct h0. *)
+    (*   - now apply F. *)
+    (*   - destruct i; cbn in *. *)
+    (*     + now apply F. *)
+    (*     + eapply F_list; eauto. *)
+    (* Defined. *)
+
+    Definition lt := lt_.
+
+    Lemma lt_strorder : StrictOrder lt.
+    Proof. Admitted.
+    (* split. *)
+    (* - intros t H. *)
+    (*   have H0 : exists u, lt t u /\ t = u by exists t. *)
+    (*   destruct H0 as (u & H' & e); induction H'; *)
+    (*     try (inversion e; fail). *)
+    (*   + injection e => e'. rewrite e' in H0. *)
+    (*     now apply StrictOrder_Irreflexive in H0. *)
+    (*   + injection e => e'. rewrite e' in H0. *)
+    (*     now apply StrictOrder_Irreflexive in H0. *)
+    (*   + injection e => _ e'. rewrite e' in H0. *)
+    (*     now apply StrictOrder_Irreflexive in H0. *)
+    (*   + injection e => e'; subst. eapply lt_list_irrefl. *)
+    (*     2: exact H0. *)
+
+    (*     intros. *)
+    (*   apply H. intros l hlt. *)
+    (*   have H0 : exists l', lt_list l l' /\ l = l' by exists l. *)
+    (*   destruct H0 as (l' & H' & e); induction H'. *)
+    (*   + injection e => e0 e1; subst. *)
+    (*     have contra : (lt u u -> False). *)
+    (*     { apply H. intro. intro. *)
+    (*     injection e' => _ e0. subst. apply IHH'; auto. *)
+    (* - intros t u v htu huv. *)
+    (*   have H0 : exists u', lt u' v /\ u = u' by exists u. *)
+    (*   destruct H0 as (u' & H' & e). clear huv. induction htu; destruct H'. *)
+    (*   (** trivial cases *) *)
+    (*   all: try now constructor. *)
+    (*   (** inconsistency in the equality *) *)
+    (*   all: try (inversion e; fail). *)
+    (*   + constructor. eapply StrictOrder_Transitive; eauto. *)
+    (*     injection e => e'; now subst. *)
+    (*   + constructor. eapply StrictOrder_Transitive; eauto. *)
+    (*     injection e => e'; now subst. *)
+    (*   + injection e => e' e''; subst. constructor. *)
+    (*     eapply StrictOrder_Transitive; eauto. *)
+    (*   + injection e => e' e''; subst; now constructor. *)
+    (*   + injection e => e' e''; subst; now constructor. *)
+    (*   + injection e => e' e''. rewrite e''. *)
+    (*     have H : lt t0 u0. *)
+    (*     {  *)
+    (*     eapply termLtFunFun2. *)
+
+    Lemma lt_compat : Proper (Logic.eq ==> Logic.eq ==> iff) lt.
+    Proof.
+      intros t u e t' u' e'. split.
+      + intros; now subst.
+      + intros; now subst.
+    Qed.
+
+    Fixpoint compare (t u : Term) : comparison :=
+      match t, u with
+      | Bound n, Bound m => OrderedNat.compare n m
+      | Bound _, Free  _ => Lt
+      | Bound _, Fun _ _ => Lt
+      | Free _ , Bound _ => Gt
+      | Free x , Free y  => OrderedString.compare x y
+      | Free _ , Fun _ _ => Lt
+      | Fun _ _, Bound _ => Gt
+      | Fun _ _, Free _ => Gt
+      | Fun x xs, Fun y ys =>
+          match OrderedString.compare x y with
+          | Eq => compare_list compare xs ys
+          | _ as v => v
+          end
+      end.
+
+    Lemma compare_spec :
+      forall t u : Term, CompareSpec (t = u) (lt t u) (lt u t) (compare t u).
+    Proof.
+      intros t u; destruct t, u; cbn.
+      - destruct (OrderedNat.compare n n0) eqn:e.
+        + constructor.
+          apply PeanoNat.Nat.compare_eq in e; now subst.
+        + constructor.
+          apply PeanoNat.Nat.compare_lt_iff in e. now constructor.
+        + constructor.
+          apply PeanoNat.Nat.compare_gt_iff in e. now constructor.
+      - do 2 constructor.
+      - do 2 constructor.
+      - do 2 constructor.
+      - have H := (OrderedString.compare_spec a a0); destruct H.
+        + constructor. now rewrite H.
+        + now do 2 constructor.
+        + now do 2 constructor.
+      - do 2 constructor.
+      - do 2 constructor.
+      - do 2 constructor.
+      - have H := (OrderedString.compare_spec a a0); destruct H.
+        + generalize dependent l0. induction l; destruct l0.
+          * constructor. now rewrite H.
+          * constructor. admit.
+          * constructor. admit.
+          * admit.
+        + now do 2 constructor.
+        + now do 2 constructor.
+    Admitted.
+
+    Definition eq_dec := @eqDec Term _.
+  End OrderedTerm.
+
+  Module SetOfTerm_ := SetFromOrdered OrderedTerm.
+  Canonical Structure SetOfTerm := SetOfTerm_.set_of_ordered.
+End ConcreteSyntaxInstances.
