theories/All.v
@@ -1,6 +1,2 @@
 From Tableaux Require Export ATPCompat.
-From Tableaux Require Export Prelude.
-From Tableaux Require Export Proofs.
-From Tableaux Require Export Semantics.
-From Tableaux Require Export Skolemization.
-From Tableaux Require Export Syntax.
+From Tableaux Require Export Core.
