theories/Prelude/All.v
@@ -1,0 +1,9 @@
+(** * Prelude.All: get everything defined in the prelude. *)
+
+From Tableaux Require Export Prelude.Init.
+From Tableaux Require Export Prelude.Classes.
+From Tableaux Require Export Prelude.Ind.
+From Tableaux Require Export Prelude.Sets.
+From Tableaux Require Export Prelude.Utils.
+From Tableaux Require Export Prelude.Atoms.
+From Tableaux Require Export Prelude.LocallyNamelessClasses.
