theories/Prelude/Atoms.v
@@ -1,0 +1,32 @@
+(** * Prelude.Atoms: the types that are suitable to make free variables *)
+
+From Tableaux Require Import Prelude.Init.
+From Tableaux Require Import Prelude.Classes.
+From Tableaux Require Import Prelude.Sets.
+
+(** ** The typeclass of atoms *)
+
+Class Atom :=
+  { atom :> Type
+  ; eq_dec_atom : EqDec atom
+  ; set_atom : set atom
+  ; isFresh : atom -> set_atom -> Prop }.
+Arguments set_atom : clear implicits.
+
+(** ** Some usual instantiations, hidden under an importable module. *)
+
+Module AtomComputationalInstances.
+  Export SetComputationalInstances.
+
+  #[global] Canonical Structure nat_atom : Atom :=
+    {| atom := nat
+    ;  eq_dec_atom := eq_dec_nat
+    ;  set_atom := SetOfNat
+    ;  isFresh := fun (x : nat) (S : SetOfNat) => ~(mem x S) |}.
+
+  #[global] Canonical Structure string_atom : Atom :=
+    {| atom := string
+    ;  eq_dec_atom := eq_dec_string
+    ;  set_atom := SetOfString
+    ;  isFresh := fun (x : string) (S : SetOfString) => ~(mem x S) |}.
+End AtomComputationalInstances.
