theories/Prelude/Classes.v
@@ -1,0 +1,77 @@
+(** * Prelude.Classes: definition of common typeclasses *)
+
+From Tableaux Require Import Prelude.Init.
+
+From Corelib Require Export Classes.RelationClasses.
+
+(** ** Typeclasses definition *)
+
+Class EqDec (A : Type) :=
+  eqDec : forall x y : A, { x = y } + { x <> y }.
+Notation "x == y" := (eqDec x y) (at level 40).
+
+Class EqBool (A : Type) :=
+  { eqb : A -> A -> bool
+  ; eqbIsEq : forall (x y : A), eqb x y = true <-> x = y }.
+
+(** ** Generic instances *)
+
+Section EqDecOtherInstances.
+  Context {A : Type} `{EqDec A}.
+
+  #[global] Instance eq_dec_list : EqDec (list A).
+  Proof using H.
+    intros xs; induction xs as [| x xs IHxs]; intro ys; destruct ys as [|y ys].
+    2,3: right; intro e; inversion e.
+    - now left.
+    - destruct (x == y).
+      2: right; intro e; injection e => e0 e1; now apply n.
+      destruct (IHxs ys).
+      + left; now rewrite e e0.
+      + right; intro e'; injection e' => e0 e1; now apply n.
+  Qed.
+End EqDecOtherInstances.
+
+Section EquivEqBoolEqDec.
+  Context (A : Type).
+
+  #[global] Instance eq_dec_from_eq_bool `{EqBool A} : EqDec A.
+  Proof using Type.
+    intros ??. destruct (eqb x y) eqn:e.
+    + left. now apply eqbIsEq in e.
+    + right. intro e'.
+      have e0 : ~(eqb x y = true).
+      { intro e0. rewrite e in e0. inversion e0. }
+      rewrite eqbIsEq in e0. now apply e0.
+  Qed.
+
+  #[global] Instance eq_bool_from_eq_dec `{EqDec A} : EqBool A.
+  Proof using Type.
+    unshelve econstructor; intros x y.
+    - exact (match x == y with
+             | left _ => true
+             | right _ => false
+             end).
+    - cbn; destruct (x == y); split; auto.
+      intro contra; inversion contra.
+  Qed.
+End EquivEqBoolEqDec.
+
+(** ** Common instances *)
+
+#[global] Instance eq_dec_nat : EqDec nat.
+Proof.
+  intros x; induction x as [|n IHn]; destruct y as [|m].
+  2,3: right; intro contra; inversion contra.
+  - now left.
+  - destruct (IHn m) as [e | ne].
+    + left; now f_equal.
+    + right; intro e. injection e => contra. now apply ne.
+Qed.
+
+#[global] Instance eq_dec_string : EqDec string.
+Proof.
+  apply eq_dec_from_eq_bool; unshelve econstructor.
+  - exact String.eqb.
+  - apply String.eqb_eq.
+Qed.
