theories/Prelude/Init.v
@@ -1,0 +1,11 @@
+(** * Prelude.Init: set basic flags and Corelib/Stdlib exports *)
+
+From Corelib Require Export ssr.ssreflect.
+
+From Stdlib Require Export Strings.String.
+From Stdlib Require Export Lists.List.
+
+Export ListNotations.
+Open Scope string_scope.
+
+Notation "#| l |" := (List.length l).
