theories/Prelude/LocallyNamelessClasses.v
@@ -1,0 +1,81 @@
+(** * Prelude.LocallyNamelessClasses: classes for locally nameless representation *)
+
+From Tableaux Require Import Init.
+From Tableaux Require Import Sets.
+From Tableaux Require Import Atoms.
+
+(** This file mainly defines the different classes (and also notations) for manipulating
+    variables in a locally nameless representation. In particular, it defines a typeclass
+    for:
+    - variable opening (i.e., instantiating a variable by a term),
+    - getting the bound variables of a term,
+    - substitution in a locally nameless environment *)
+
+(** ** Variable opening: replacing a bound variable with an atom *)
+Class Opening (A B : Type) :=
+  varOpening : nat -> A -> B -> B.
+Arguments varOpening {_ _ _} _ _ _.
+Notation "t { n \to x }" := (varOpening n x t) (at level 3).
+
+(** ** Variable substitution: replacing a free variable with something *)
+Section Substitution.
+  Context `{set_nat : set nat}.
+
+  Class BV (A : Type) :=
+    bv : A -> set_nat.
+  Arguments bv {_ _}.
+
+  Definition isLocallyClosed {A : Type} `{BV A} (x : A) :=
+    is_empty (bv x).
+
+  Class Substitution (X : Atom) (A : Type) `{BV A} :=
+    { subst :> X -> A
+    ; isSubst : forall (x : X), isLocallyClosed (subst x) }.
+
+  Class Subst {X : Atom} (A B : Type) `{BV B} :=
+    substitute : A -> Substitution X B -> A.
+  Arguments substitute {_ _ _ _ _} _ _.
+End Substitution.
+
+Notation "x @[ sigma ]" := (substitute x sigma) (at level 3).
+
+(** ** Further free instances of [Subst]. *)
+Section SubstInstances.
+  Context `{set_nat : set nat}.
+
+  #[global] Instance subst_list {X : Atom} {A B : Type} `{H : BV B} `{Subst A B} :
+    Subst (list A) B :=
+    fun xs sigma =>
+      (fix F (xs : list A) : list A :=
+         match xs with
+         | [] => []
+         | x :: xs => x@[sigma] :: F xs
+         end) xs.
+End SubstInstances.
+
+(** ** Free variable and free-variable closedness *)
+Section FreeVariables.
+  Context {var : Atom}.
+
+  Let set_var := set_atom var.
+
+  Class FV (A : Type) :=
+    fv : A -> set_var.
+
+  Definition isClosed {A : Type} `{FV A} (x : A) :=
+    is_empty (fv x).
+End FreeVariables.
+
+(** ** Further free instances of [FV]. *)
+Section FVInstances.
+  Context {var : Atom}.
+
+  Let set_var := set_atom var.
+
+  #[global] Instance fv_list {A : Type} `{@FV var A} : @FV var (list A) :=
+    fix F (xs : list A) : set_var :=
+      match xs with
+      | [] => empty_set
+      | x :: xs => (fv x) \union (F xs)
+      end.
+End FVInstances.
