theories/Prelude/Utils.v
@@ -1,0 +1,13 @@
+(** * Prelude.Utils: some utility functions / lemmas *)
+
+Definition option_get {A : Type} (def : A) (x : option A) : A :=
+  match x with
+  | None => def
+  | Some x => x
+  end.
+
+Definition bind {A B : Type} (x : option A) (f : A -> option B) : option B :=
+  match x with
+  | Some x => f x
+  | None => None
+  end.
